Weidenbach_Book/IsaSAT/IsaSAT_Initialisation.thy
@@ -2089,7 +2089,7 @@ definition finalise_init_code :: \<open>opts \<Rightarrow> twl_st_wl_heur_init \
     (\<lambda>(M', N', D', Q', W', ((ns, m, fst_As, lst_As, next_search), to_remove), \<phi>, clvls, cach,
        lbd, vdom, _, lcount, mark). do {
      ASSERT(lst_As \<noteq> None \<and> fst_As \<noteq> None);
-     let init_stats = (0::64 word, 0::64 word, 0::64 word, 0::64 word, 0::64 word, 0::64 word, 0::64 word, ema_fast_init);
+     let init_stats = (0::64 word, 0::64 word, 0::64 word, 0::64 word, 0::64 word, 0::64 word, 0::64 word,0::64 word, ema_fast_init);
      let fema = ema_init (opts_fema opts);
      let sema = ema_init (opts_sema opts);
      let ccount = restart_info_init;
