Weidenbach_Book/IsaSAT/IsaSAT_Inprocessing_LLVM.thy
@@ -1,0 +1,18 @@
+theory IsaSAT_Inprocessing_LLVM
+  imports IsaSAT_Setup_LLVM
+    IsaSAT_Restart_Inprocessing
+begin
+
+sepref_register isa_simplify_clauses_with_unit_st2
+sepref_def isa_simplify_clauses_with_unit_st2_code
+  is isa_simplify_clauses_with_unit_st2
+  :: \<open>isasat_bounded_assn\<^sup>d \<rightarrow>\<^sub>a isasat_bounded_assn\<close>
+  unfolding isa_simplify_clauses_with_unit_st2_alt_def
+  by sepref
+
+experiment
+begin
+  export_llvm isa_simplify_clauses_with_unit_st2_code
+end
+
+end
