Weidenbach_Book/IsaSAT/IsaSAT_Restart_LLVM.thy
@@ -3,15 +3,6 @@ imports IsaSAT_Restart IsaSAT_Restart_Heuristics_LLVM IsaSAT_Garbage_Collect_LLV
   IsaSAT_Other_LLVM IsaSAT_Propagate_Conflict_LLVM
 begin
 
-sepref_register update_all_phases
-
-sepref_def update_all_phases_impl
-  is \<open>update_all_phases\<close>
-  :: \<open>isasat_bounded_assn\<^sup>d \<rightarrow>\<^sub>a isasat_bounded_assn\<close>
-  unfolding update_all_phases_def
-  by sepref
-
-
 sepref_register mark_to_delete_clauses_wl_D_heur
 
 sepref_def MINIMUM_DELETION_LBD_impl
@@ -25,66 +16,14 @@ sepref_def MINIMUM_DELETION_LBD_impl
 sepref_register delete_index_and_swap mop_mark_garbage_heur mop_mark_garbage_heur3
   mop_access_lit_in_clauses_heur
 
-sepref_def mark_to_delete_clauses_wl_D_heur_fast_impl
-  is \<open>mark_to_delete_clauses_wl_D_heur\<close>
-  :: \<open>[\<lambda>S. length (get_clauses_wl_heur S) \<le> sint64_max]\<^sub>a isasat_bounded_assn\<^sup>d \<rightarrow> isasat_bounded_assn\<close>
-  unfolding mark_to_delete_clauses_wl_D_heur_def
-    access_vdom_at_def[symmetric] length_avdom_def[symmetric]
-    get_the_propagation_reason_heur_def[symmetric]
-    clause_is_learned_heur_def[symmetric]
-    clause_lbd_heur_def[symmetric]
-    access_length_heur_def[symmetric]
-    mark_to_delete_clauses_wl_D_heur_is_Some_iff
-    marked_as_used_st_def[symmetric] if_conn(4)
-    fold_tuple_optimizations
-    mop_arena_lbd_st_def[symmetric]
-    mop_marked_as_used_st_def[symmetric]
-    mop_arena_status_st_def[symmetric]
-    mop_arena_length_st_def[symmetric]
-  supply [[goals_limit = 1]] of_nat_snat[sepref_import_param]
-      length_avdom_def[symmetric, simp] access_vdom_at_def[simp]
-  apply (rewrite in \<open>let _ = \<hole> in _\<close> short_circuit_conv)+
-  apply (rewrite at \<open>_ > \<hole>\<close> unat_const_fold[where 'a=2])
-  apply (annot_snat_const \<open>TYPE(64)\<close>)
-  by sepref
-
 
 sepref_register cdcl_twl_full_restart_wl_prog_heur
-
-sepref_def cdcl_twl_full_restart_wl_prog_heur_fast_code
-  is \<open>cdcl_twl_full_restart_wl_prog_heur\<close>
-  :: \<open>[\<lambda>S. length (get_clauses_wl_heur S) \<le> sint64_max]\<^sub>a isasat_bounded_assn\<^sup>d \<rightarrow> isasat_bounded_assn\<close>
-  unfolding cdcl_twl_full_restart_wl_prog_heur_def
-  supply [[goals_limit = 1]]
-  by sepref
 
 sepref_def cdcl_twl_restart_wl_heur_fast_code
   is \<open>cdcl_twl_restart_wl_heur\<close>
   :: \<open>[\<lambda>S. length (get_clauses_wl_heur S) \<le> sint64_max]\<^sub>a isasat_bounded_assn\<^sup>d \<rightarrow> isasat_bounded_assn\<close>
   unfolding cdcl_twl_restart_wl_heur_def
   supply [[goals_limit = 1]]
-  by sepref
-
-
-sepref_def cdcl_twl_full_restart_wl_D_GC_heur_prog_fast_code
-  is \<open>cdcl_twl_full_restart_wl_D_GC_heur_prog\<close>
-  :: \<open>[\<lambda>S. length (get_clauses_wl_heur S) \<le> sint64_max \<and> learned_clss_count S \<le> uint64_max]\<^sub>a
-     isasat_bounded_assn\<^sup>d \<rightarrow> isasat_bounded_assn\<close>
-  supply [[goals_limit = 1]]
-  unfolding cdcl_twl_full_restart_wl_D_GC_heur_prog_def
-  apply (annot_unat_const \<open>TYPE(32)\<close>)
-  by sepref
-
-sepref_register restart_required_heur cdcl_twl_restart_wl_heur
-
-sepref_def restart_prog_wl_D_heur_fast_code
-  is \<open>uncurry4 (restart_prog_wl_D_heur)\<close>
-  :: \<open>[\<lambda>((((S, _), _), n), _). isasat_fast_relaxed2 S n]\<^sub>a
-      isasat_bounded_assn\<^sup>d *\<^sub>a uint64_nat_assn\<^sup>k  *\<^sub>a uint64_nat_assn\<^sup>k  *\<^sub>a uint64_nat_assn\<^sup>k *\<^sub>a
-        bool1_assn\<^sup>k \<rightarrow> isasat_bounded_assn \<times>\<^sub>a uint64_nat_assn \<times>\<^sub>a uint64_nat_assn \<times>\<^sub>a uint64_nat_assn\<close>
-  unfolding restart_prog_wl_D_heur_def isasat_fast_relaxed_def isasat_fast_relaxed2_def
-  supply [[goals_limit = 1]]
-  apply (annot_unat_const \<open>TYPE(64)\<close>)
   by sepref
 
 definition isasat_fast_bound where
@@ -106,49 +45,6 @@ lemma isasat_fast_alt_def: \<open>isasat_fast S = (length_clauses_heur S \<le> 9
 
 sepref_register isasat_fast
 
-sepref_def isasat_fast_code
-  is \<open>RETURN o isasat_fast\<close>
-  :: \<open>[\<lambda>S. isasat_fast_relaxed S]\<^sub>a isasat_bounded_assn\<^sup>k \<rightarrow> bool1_assn\<close>
-  unfolding isasat_fast_alt_def isasat_fast_relaxed_def
-  apply (rewrite at \<open>_ < \<hole>\<close> unat_const_fold[where 'a=64])+
-  unfolding all_count_learned[symmetric] clss_size_allcount_alt_def
-  supply [[goals_limit = 1]]
-  apply (annot_snat_const \<open>TYPE(64)\<close>)
-  by sepref
-
-lemma cdcl_twl_stgy_restart_prog_bounded_wl_heurI1:
-  assumes
-    \<open>isasat_fast a1'b\<close>
-    \<open>learned_clss_count a2'e \<le> Suc (learned_clss_count a1'b)\<close>
-  shows \<open>learned_clss_count a2'e \<le> uint64_max\<close>
-  using assms
-  by (auto simp: isasat_fast_def)
-
-lemma cdcl_twl_stgy_restart_prog_bounded_wl_heurI2:
-  \<open>isasat_fast x \<Longrightarrow> learned_clss_count x \<le> uint64_max\<close>
-  by (auto simp: isasat_fast_def)
-
-
-lemma cdcl_twl_stgy_restart_prog_bounded_wl_heurI3:
-  assumes
-    \<open>isasat_fast S\<close>
-    \<open>length (get_clauses_wl_heur T) \<le> length (get_clauses_wl_heur S)\<close>
-    \<open>learned_clss_count T \<le> (learned_clss_count S)\<close>
-  shows \<open>isasat_fast T\<close>
-  using assms
-  by (auto simp: isasat_fast_def)
-
-sepref_register cdcl_twl_stgy_restart_prog_bounded_wl_heur
-sepref_def cdcl_twl_stgy_restart_prog_wl_heur_fast_code
-  is \<open>cdcl_twl_stgy_restart_prog_bounded_wl_heur\<close>
-  :: \<open>[\<lambda>S. isasat_fast S]\<^sub>a isasat_bounded_assn\<^sup>d \<rightarrow> bool1_assn \<times>\<^sub>a isasat_bounded_assn\<close>
-  unfolding cdcl_twl_stgy_restart_prog_bounded_wl_heur_def
-  supply [[goals_limit = 1]] isasat_fast_countD[dest]
-  supply [intro] = cdcl_twl_stgy_restart_prog_bounded_wl_heurI2
-  supply [sepref_bounds_simps del] = uint32_max_def sint32_max_def uint64_max_def sint64_max_def
-  apply (annot_unat_const \<open>TYPE(64)\<close>)
-  by sepref
-
 
 experiment
 begin
@@ -162,9 +58,7 @@ begin
     upper_restart_bound_not_reached_fast_impl
     minimum_number_between_restarts_impl
     restart_required_heur_fast_code
-    cdcl_twl_full_restart_wl_D_GC_heur_prog_fast_code
     cdcl_twl_restart_wl_heur_fast_code
-    cdcl_twl_full_restart_wl_prog_heur_fast_code
     cdcl_twl_local_restart_wl_D_heur_fast_code
    get_conflict_wl_is_None_fast_code
 end
